gravy_test/regression/infeasible_code/infeasiblecode001.bpl
@@ -11,19 +11,21 @@ const unique $type : Field javaType;
 const unique $alloc : Field bool;
 const { :SourceLocation "Object.java",-1,-1,-1,-1 } unique java.lang.Object : javaType extends  complete;
 const { :SourceLocation "InfeasibleCode01.java",-1,-1,-1,-1 } unique InfeasibleCode01 : javaType extends  unique java.lang.Object complete;
-const { :SourceLocation "Serializable.java",-1,-1,-1,-1 } unique java.io.Serializable : javaType extends  unique java.lang.Object complete;
-const { :SourceLocation "Comparable.java",-1,-1,-1,-1 } unique java.lang.Comparable : javaType extends  unique java.lang.Object complete;
-const { :SourceLocation "CharSequence.java",-1,-1,-1,-1 } unique java.lang.CharSequence : javaType extends  unique java.lang.Object complete;
-const { :SourceLocation "String.java",-1,-1,-1,-1 } unique java.lang.String : javaType extends  unique java.lang.Object, unique java.lang.Comparable, unique java.io.Serializable, unique java.lang.CharSequence complete;
 const { :SourceLocation "Appendable.java",-1,-1,-1,-1 } unique java.lang.Appendable : javaType extends  unique java.lang.Object complete;
-const { :SourceLocation "AbstractStringBuilder.java",-1,-1,-1,-1 } unique java.lang.AbstractStringBuilder : javaType extends  unique java.lang.Object, unique java.lang.Appendable, unique java.lang.CharSequence complete;
-const { :SourceLocation "StringBuffer.java",-1,-1,-1,-1 } unique java.lang.StringBuffer : javaType extends  unique java.lang.AbstractStringBuilder, unique java.io.Serializable, unique java.lang.CharSequence complete;
+const { :SourceLocation "CharSequence.java",-1,-1,-1,-1 } unique java.lang.CharSequence : javaType extends  unique java.lang.Object complete;
+const { :SourceLocation "AbstractStringBuilder.java",-1,-1,-1,-1 } unique java.lang.AbstractStringBuilder : javaType extends  unique java.lang.CharSequence, unique java.lang.Appendable, unique java.lang.Object complete;
+const { :SourceLocation "Serializable.java",-1,-1,-1,-1 } unique java.io.Serializable : javaType extends  unique java.lang.Object complete;
+const { :SourceLocation "StringBuffer.java",-1,-1,-1,-1 } unique java.lang.StringBuffer : javaType extends  unique java.lang.CharSequence, unique java.lang.AbstractStringBuilder, unique java.io.Serializable complete;
+const { :SourceLocation "Comparable.java",-1,-1,-1,-1 } unique java.lang.Comparable : javaType extends  unique java.lang.Object complete;
+const { :SourceLocation "String.java",-1,-1,-1,-1 } unique java.lang.String : javaType extends  unique java.lang.Comparable, unique java.lang.CharSequence, unique java.lang.Object, unique java.io.Serializable complete;
+const unique $StringConst0 : ref extends  complete;
 const { :SourceLocation "AutoCloseable.java",-1,-1,-1,-1 } unique java.lang.AutoCloseable : javaType extends  unique java.lang.Object complete;
-const { :SourceLocation "Closeable.java",-1,-1,-1,-1 } unique java.io.Closeable : javaType extends  unique java.lang.Object, unique java.lang.AutoCloseable complete;
+const { :SourceLocation "Closeable.java",-1,-1,-1,-1 } unique java.io.Closeable : javaType extends  unique java.lang.AutoCloseable, unique java.lang.Object complete;
 const { :SourceLocation "Flushable.java",-1,-1,-1,-1 } unique java.io.Flushable : javaType extends  unique java.lang.Object complete;
-const { :SourceLocation "OutputStream.java",-1,-1,-1,-1 } unique java.io.OutputStream : javaType extends  unique java.io.Closeable, unique java.io.Flushable, unique java.lang.Object complete;
+const { :SourceLocation "OutputStream.java",-1,-1,-1,-1 } unique java.io.OutputStream : javaType extends  unique java.io.Flushable, unique java.io.Closeable, unique java.lang.Object complete;
 const { :SourceLocation "FilterOutputStream.java",-1,-1,-1,-1 } unique java.io.FilterOutputStream : javaType extends  unique java.io.OutputStream complete;
-const { :SourceLocation "PrintStream.java",-1,-1,-1,-1 } unique java.io.PrintStream : javaType extends  unique java.io.Closeable, unique java.io.FilterOutputStream, unique java.lang.Appendable complete;
+const { :SourceLocation "PrintStream.java",-1,-1,-1,-1 } unique java.io.PrintStream : javaType extends  unique java.lang.Appendable, unique java.io.Closeable, unique java.io.FilterOutputStream complete;
+const unique $StringConst1 : ref extends  complete;
 var $heap : $heap_type;
 var $intArrayType : javaType;
 var $charArrayType : javaType;
@@ -37,8 +39,6 @@ var $refArrHeap : refArrHeap_type;
 var $realArrHeap : realArrHeap_type;
 var $intArrHeap : intArrHeap_type;
 var java.io.PrintStream$java.lang.System$err236 : ref;
-var $DUMMYVAR__0 : ref;
-var $DUMMYVAR__1 : ref;
 function $arrayType(t:javaType) returns ($ret:javaType);
 function $intToReal(x:int) returns ($ret:real);
 function $intToBool(x:int) returns ($ret:bool) { (if x == 0 then false else true) }
@@ -54,20 +54,15 @@ function $xorInt(x:int, y:int) returns ($ret:int);
 function $shlInt(x:int, y:int) returns ($ret:int);
 function $ushrInt(x:int, y:int) returns ($ret:int);
 function $shrInt(x:int, y:int) returns ($ret:int);
-procedure java.lang.Object$java.lang.Object$clone$43($this:ref) returns ($other:ref)    modifies $heap;{
-    havoc $other;
-    assume !$heap[$other,$alloc];
-    $heap := $heap[$other,$alloc := true];
-    assume $other != $null;
-    $heap := $heap[$other,$type := $heap[$this,$type]];
-}
+procedure $new(obj_type:javaType) returns ($obj:ref);    ensures $obj != $null;    ensures $heap[$obj,$alloc] == true;    requires $heap[$obj,$alloc] == false;        ensures $heap[$obj,$type] == obj_type;
 
+procedure java.lang.Object$java.lang.Object$clone$43($this:ref) returns ($other:ref);    ensures $heap[$other,$alloc] == true;        ensures $heap[$other,$type] == $heap[$this,$type];    ensures $other != $null;
 
-procedure int$java.lang.String$compareTo$87($this:ref, $other:ref) returns ($return:int);    ensures ($this == $other ==> $return == 1) && ($this != $other ==> $return == 0);    
+procedure int$java.lang.String$compareTo$87($this:ref, $other:ref) returns ($return:int);        ensures ($this == $other ==> $return == 1) && ($this != $other ==> $return == 0);
 
 procedure int$InfeasibleCode01$infeasible0$1889($this:ref, $in_parameter__0:ref) returns ($return:int, $exception:ref);    modifies $intArrHeap;
 
-procedure int$InfeasibleCode01$infeasible1$1890($this:ref, $in_parameter__0:ref) returns ($return:int, $exception:ref);    modifies $heap;
+procedure int$InfeasibleCode01$infeasible1$1890($this:ref, $in_parameter__0:ref) returns ($return:int, $exception:ref);    
 
 procedure int$java.lang.Object$hashCode$41($this:ref) returns ($return:int, $exception:ref);    
 
@@ -87,7 +82,7 @@ procedure void$InfeasibleCode01$infeasible3$1892($this:ref, $in_parameter__0:int
 
 procedure boolean$InfeasibleCode01$infeasible4$1893($this:ref, $in_parameter__0:ref) returns ($return:int, $exception:ref);    
 
-procedure void$InfeasibleCode01$infeasible5$1894($this:ref) returns ($exception:ref);    modifies $heap, $stringSizeHeap;
+procedure void$InfeasibleCode01$infeasible5$1894($this:ref) returns ($exception:ref);    modifies $stringSizeHeap;
 
 procedure int$InfeasibleCode01$infeasible6$1895($this:ref, $in_parameter__0:ref) returns ($return:int, $exception:ref);    
 
@@ -97,18 +92,16 @@ procedure void$java.lang.Object$$la$init$ra$$38($this:ref) returns ($exception:r
 
 implementation int$InfeasibleCode01$infeasible0$1889($this:ref, $in_parameter__0:ref) returns ($return:int, $exception:ref){
     
-var temp$04 : ref;    
-var temp$26 : int;    
+var temp$37 : ref;    
+var temp$48 : int;    
 var i3 : int;    
 var this1 : ref;    
-var temp$37 : ref;    
-var $ex_return : bool;    
 var temp$15 : int;    
-var temp$48 : int;    
-var arr2 : ref;    
-var temp$59 : int;
+var temp$59 : int;    
+var temp$04 : ref;    
+var temp$26 : int;    
+var arr2 : ref;
     assume $this != $null;
-    $ex_return := false;
     this1 := $this;
     arr2 := $in_parameter__0;
     assert { :SourceLocation "InfeasibleCode01.java",28,28,3,21 } arr2 != $null;
@@ -130,67 +123,46 @@ var temp$59 : int;
 implementation int$InfeasibleCode01$infeasible1$1890($this:ref, $in_parameter__0:ref) returns ($return:int, $exception:ref){
     
 var $fakelocal_2 : ref;    
-var $fakelocal_1 : ref;    
-var temp$012 : int;    
-var temp$315 : ref;    
-var temp$416 : ref;    
-var temp$517 : int;    
-var $fakelocal_0 : ref;    
 var temp$113 : ref;    
-var temp$214 : ref;    
+var temp$416 : ref;    
+var o11 : ref;    
+var $fakelocal_0 : ref;    
 var this10 : ref;    
-var $ex_return : bool;    
-var o11 : ref;
+var temp$315 : ref;    
+var temp$012 : int;    
+var temp$214 : ref;    
+var temp$517 : int;    
+var $fakelocal_1 : ref;
     assume $this != $null;
-    $ex_return := false;
     this10 := $this;
     o11 := $in_parameter__0;
     if (o11 != $null) {
+        assert { :SourceLocation "InfeasibleCode01.java",34,34,7,13 } true;
         goto block1;
+    } else {
+        assert { :SourceLocation "InfeasibleCode01.java",34,34,7,13 } true;
     }
     goto block2;
   block1:
     assert { :SourceLocation "InfeasibleCode01.java",34,34,7,13 } o11 != $null;
-    if ($heap[o11,$type] <: java.lang.String && java.lang.String <: $heap[o11,$type]) {
-        call temp$012, $exception := int$java.lang.Object$hashCode$41(o11);
-    }
-    if ($heap[o11,$type] <: java.lang.Object && java.lang.Object <: $heap[o11,$type]) {
-        call temp$012, $exception := int$java.lang.Object$hashCode$41(o11);
-    }
+    call temp$012, $exception := int$java.lang.Object$hashCode$41(o11);
     $return := temp$012;
     return;
   block2:
     temp$113 := java.io.PrintStream$java.lang.System$err236;
-    havoc $fakelocal_0;
-    assume !$heap[$fakelocal_0,$alloc];
-    $heap := $heap[$fakelocal_0,$alloc := true];
-    assume $fakelocal_0 != $null;
-    $heap := $heap[$fakelocal_0,$type := java.lang.StringBuffer];
+    call $fakelocal_0 := $new(java.lang.StringBuffer);
     temp$214 := $fakelocal_0;
     call $exception := void$java.lang.StringBuffer$$la$init$ra$$685(temp$214);
     assert { :SourceLocation "InfeasibleCode01.java",37,37,22,53 } o11 != $null;
-    if ($heap[o11,$type] <: java.lang.String && java.lang.String <: $heap[o11,$type]) {
-        call temp$315, $exception := java.lang.String$java.lang.Object$toString$44(o11);
-    }
-    if ($heap[o11,$type] <: java.lang.Object && java.lang.Object <: $heap[o11,$type]) {
-        call temp$315, $exception := java.lang.String$java.lang.Object$toString$44(o11);
-    }
+    call temp$315, $exception := java.lang.String$java.lang.Object$toString$44(o11);
     assert { :SourceLocation "InfeasibleCode01.java",37,37,22,53 } temp$214 != $null;
-    if ($heap[temp$214,$type] <: java.lang.StringBuffer && java.lang.StringBuffer <: $heap[temp$214,$type]) {
-        call $fakelocal_1, $exception := java.lang.StringBuffer$java.lang.StringBuffer$append$701(temp$214, temp$315);
-    }
+    call $fakelocal_1, $exception := java.lang.StringBuffer$java.lang.StringBuffer$append$701(temp$214, temp$315);
     assert { :SourceLocation "InfeasibleCode01.java",37,37,22,53 } temp$214 != $null;
-    if ($heap[temp$214,$type] <: java.lang.StringBuffer && java.lang.StringBuffer <: $heap[temp$214,$type]) {
-        call $fakelocal_2, $exception := java.lang.StringBuffer$java.lang.StringBuffer$append$701(temp$214, $DUMMYVAR__0);
-    }
+    call $fakelocal_2, $exception := java.lang.StringBuffer$java.lang.StringBuffer$append$701(temp$214, $StringConst0);
     assert { :SourceLocation "InfeasibleCode01.java",37,37,22,53 } temp$214 != $null;
-    if ($heap[temp$214,$type] <: java.lang.StringBuffer && java.lang.StringBuffer <: $heap[temp$214,$type]) {
-        call temp$416, $exception := java.lang.String$java.lang.StringBuffer$toString$738(temp$214);
-    }
+    call temp$416, $exception := java.lang.String$java.lang.StringBuffer$toString$738(temp$214);
     assert { :SourceLocation "InfeasibleCode01.java",37,37,22,53 } temp$113 != $null;
-    if ($heap[temp$113,$type] <: java.io.PrintStream && java.io.PrintStream <: $heap[temp$113,$type]) {
-        call $exception := void$java.io.PrintStream$println$217(temp$113, temp$416);
-    }
+    call $exception := void$java.io.PrintStream$println$217(temp$113, temp$416);
     temp$517 := 2;
     $return := temp$517;
     return;
@@ -199,17 +171,15 @@ var o11 : ref;
 
 implementation void$InfeasibleCode01$infeasible2$1891($this:ref, $in_parameter__0:ref) returns ($exception:ref){
     
-var i20 : int;    
-var temp$122 : ref;    
-var $ex_return : bool;    
-var arr19 : ref;    
-var temp$223 : int;    
-var this18 : ref;    
-var temp$425 : int;    
 var temp$324 : int;    
-var temp$021 : int;
+var temp$223 : int;    
+var temp$122 : ref;    
+var i20 : int;    
+var temp$021 : int;    
+var arr19 : ref;    
+var temp$425 : int;    
+var this18 : ref;
     assume $this != $null;
-    $ex_return := false;
     this18 := $this;
     arr19 := $in_parameter__0;
     i20 := 0;
@@ -217,7 +187,10 @@ var temp$021 : int;
     assert { :SourceLocation "InfeasibleCode01.java",42,42,17,29 } arr19 != $null;
     temp$021 := $arrSizeHeap[arr19];
     if (i20 <= temp$021) {
+        assert { :SourceLocation "InfeasibleCode01.java",42,42,17,29 } true;
         goto block4;
+    } else {
+        assert { :SourceLocation "InfeasibleCode01.java",42,42,17,29 } true;
     }
     goto block5;
   block4:
@@ -236,25 +209,26 @@ var temp$021 : int;
 
 implementation void$InfeasibleCode01$infeasible3$1892($this:ref, $in_parameter__0:int, $in_parameter__1:int) returns ($exception:ref){
     
-var temp$433 : int;    
-var this26 : ref;    
-var a27 : int;    
-var $ex_return : bool;    
+var temp$130 : int;    
 var temp$332 : int;    
-var temp$029 : int;    
-var temp$231 : int;    
+var a27 : int;    
 var temp$534 : int;    
+var temp$029 : int;    
+var this26 : ref;    
+var temp$433 : int;    
 var b28 : int;    
-var temp$130 : int;
+var temp$231 : int;
     assume $this != $null;
-    $ex_return := false;
     this26 := $this;
     a27 := $in_parameter__0;
     b28 := $in_parameter__1;
     temp$029 := 1;
     b28 := temp$029;
     if (a27 > 0) {
+        assert { :SourceLocation "InfeasibleCode01.java",49,49,7,9 } true;
         goto block6;
+    } else {
+        assert { :SourceLocation "InfeasibleCode01.java",49,49,7,9 } true;
     }
     goto block7;
   block6:
@@ -266,7 +240,10 @@ var temp$130 : int;
     temp$332 := 1 div b28;
     b28 := temp$332;
     if (a27 <= 0) {
+        assert { :SourceLocation "InfeasibleCode01.java",51,51,7,10 } true;
         goto block8;
+    } else {
+        assert { :SourceLocation "InfeasibleCode01.java",51,51,7,10 } true;
     }
     goto block9;
   block8:
@@ -281,31 +258,25 @@ var temp$130 : int;
 
 implementation boolean$InfeasibleCode01$infeasible4$1893($this:ref, $in_parameter__0:ref) returns ($return:int, $exception:ref){
     
-var $ex_return : bool;    
-var temp$340 : int;    
-var temp$037 : ref;    
 var this35 : ref;    
+var o36 : ref;    
 var temp$138 : ref;    
-var temp$239 : int;    
-var o36 : ref;
+var temp$037 : ref;    
+var temp$340 : int;    
+var temp$239 : int;
     assume $this != $null;
-    $ex_return := false;
     this35 := $this;
     o36 := $in_parameter__0;
     temp$037 := java.io.PrintStream$java.lang.System$err236;
     assert { :SourceLocation "InfeasibleCode01.java",55,55,3,35 } o36 != $null;
-    if ($heap[o36,$type] <: java.lang.String && java.lang.String <: $heap[o36,$type]) {
-        call temp$138, $exception := java.lang.String$java.lang.Object$toString$44(o36);
-    }
-    if ($heap[o36,$type] <: java.lang.Object && java.lang.Object <: $heap[o36,$type]) {
-        call temp$138, $exception := java.lang.String$java.lang.Object$toString$44(o36);
-    }
+    call temp$138, $exception := java.lang.String$java.lang.Object$toString$44(o36);
     assert { :SourceLocation "InfeasibleCode01.java",55,55,3,35 } temp$037 != $null;
-    if ($heap[temp$037,$type] <: java.io.PrintStream && java.io.PrintStream <: $heap[temp$037,$type]) {
-        call $exception := void$java.io.PrintStream$println$217(temp$037, temp$138);
-    }
+    call $exception := void$java.io.PrintStream$println$217(temp$037, temp$138);
     if (o36 == $null) {
+        assert { :SourceLocation "InfeasibleCode01.java",56,56,7,13 } true;
         goto block10;
+    } else {
+        assert { :SourceLocation "InfeasibleCode01.java",56,56,7,13 } true;
     }
     goto block11;
   block10:
@@ -321,33 +292,28 @@ var o36 : ref;
 
 implementation void$InfeasibleCode01$infeasible5$1894($this:ref) returns ($exception:ref){
     
-var temp$144 : ref;    
-var $ex_return : bool;    
-var $fakelocal_0 : ref;    
 var temp$043 : int;    
+var test42 : ref;    
 var this41 : ref;    
-var test42 : ref;
+var $fakelocal_0 : ref;    
+var temp$144 : ref;
     assume $this != $null;
-    $ex_return := false;
     this41 := $this;
-    havoc $fakelocal_0;
-    assume !$heap[$fakelocal_0,$alloc];
-    $heap := $heap[$fakelocal_0,$alloc := true];
-    assume $fakelocal_0 != $null;
-    $heap := $heap[$fakelocal_0,$type := java.lang.String];
+    call $fakelocal_0 := $new(java.lang.String);
     $stringSizeHeap := $stringSizeHeap[$fakelocal_0 := 8];
     test42 := $fakelocal_0;
     temp$043 := $stringSizeHeap[test42];
     if (temp$043 == 3) {
+        assert { :SourceLocation "InfeasibleCode01.java",64,64,7,22 } true;
         goto block12;
+    } else {
+        assert { :SourceLocation "InfeasibleCode01.java",64,64,7,22 } true;
     }
     goto block13;
   block12:
     temp$144 := java.io.PrintStream$java.lang.System$err236;
     assert { :SourceLocation "InfeasibleCode01.java",65,65,4,37 } temp$144 != $null;
-    if ($heap[temp$144,$type] <: java.io.PrintStream && java.io.PrintStream <: $heap[temp$144,$type]) {
-        call $exception := void$java.io.PrintStream$println$217(temp$144, $DUMMYVAR__1);
-    }
+    call $exception := void$java.io.PrintStream$println$217(temp$144, $StringConst1);
   block13:
     return;
 }
@@ -355,18 +321,16 @@ var test42 : ref;
 
 implementation int$InfeasibleCode01$infeasible6$1895($this:ref, $in_parameter__0:ref) returns ($return:int, $exception:ref){
     
+var temp$653 : int;    
+var temp$350 : ref;    
+var temp$148 : int;    
+var arr46 : ref;    
 var temp$451 : int;    
 var temp$552 : int;    
-var arr46 : ref;    
-var temp$653 : int;    
-var temp$148 : int;    
-var temp$249 : int;    
-var temp$047 : ref;    
 var this45 : ref;    
-var $ex_return : bool;    
-var temp$350 : ref;
+var temp$047 : ref;    
+var temp$249 : int;
     assume $this != $null;
-    $ex_return := false;
     this45 := $this;
     arr46 := $in_parameter__0;
     temp$047 := arr46;
@@ -386,10 +350,8 @@ var temp$350 : ref;
 
 implementation void$InfeasibleCode01$$la$init$ra$$1896($this:ref) returns ($exception:ref){
     
-var this54 : ref;    
-var $ex_return : bool;
+var this54 : ref;
     assume $this != $null;
-    $ex_return := false;
     this54 := $this;
     call $exception := void$java.lang.Object$$la$init$ra$$38(this54);
     return;
